Seq module and monadic notation for option in Util

Model/Model.v
@@ -1,107 +1,204 @@
+Require Import Lia.
 Require Import Seq.
 Declare Scope model_scope.
+Open Scope model_scope.
 
-Module Type TS.
-  Parameter State : Set.
-  Parameter Action : Set.
-  Parameter Atomic : Set.
-  Parameter start : State.
-  Parameter transition : State -> Action -> option State.
-  Parameter label : State -> Atomic -> bool.
-End TS.
+Parameter State : Set.
+Parameter Action : Set.
+Parameter Atomic : Set.
+Parameter start : State.
+Parameter transition : State -> Action -> option State.
+Parameter label : State -> Atomic -> bool.
 
-Module Theory (ts : TS).
-  Import ts.
+Inductive StateFormula : Set :=
+  | Always : StateFormula
+  | Atom : Atomic -> StateFormula
+  | Not : StateFormula -> StateFormula
+  | And : StateFormula -> StateFormula -> StateFormula
+  | Exists : PathFormula -> StateFormula
+  | Forall : PathFormula -> StateFormula
+with PathFormula : Set :=
+  | Next : StateFormula -> PathFormula
+  | Globally : StateFormula -> PathFormula
+  | Eventually : StateFormula -> PathFormula
+  | Until : StateFormula -> StateFormula -> PathFormula.
 
-  Inductive StateFormula : Set :=
-    | Always : StateFormula
-    | Atom : Atomic -> StateFormula
-    | And : StateFormula -> StateFormula -> StateFormula
-    | Not : StateFormula -> StateFormula
-    | One : PathFormula -> StateFormula
-    | All : PathFormula -> StateFormula
-  with PathFormula : Set :=
-    | Next : StateFormula -> PathFormula
-    | Globally : StateFormula -> PathFormula
-    | Eventually : StateFormula -> PathFormula
-    | Until : StateFormula -> StateFormula -> PathFormula.
+Notation "! x" := (not x) (at level 75, right associativity) : model_scope.
+Notation "x & y" := (conj x y) (at level 80, right associativity) : model_scope.
+Notation "'Exists' x" := (Exists x) (at level 65, right associativity) : model_scope.
+Notation "'Forall' x" := (Forall x) (at level 65, right associativity) : model_scope.
 
-  Notation "'Exists' x" := (some x) (at level 65, right associativity) : model_scope.
-  Notation "'Forall' x" := (every x) (at level 65, right associativity) : model_scope.
-  Notation "x /\ y" := (conj x y) (at level 80, right associativity) : model_scope.
-  Notation "~ x" := (not x) (at level 75, right associativity) : model_scope.
-  Notation "'X x" := (next x) (at level 65, right associativity) : model_scope.
-  Notation "'A' x" := (always x) (at level 65, right associativity) : model_scope.
-  Notation "'E' x" := (eventually x) (at level 65, right associativity) : model_scope.
-  Notation "x 'U' y" := (until x y) (at level 60, right associativity) : model_scope.
+Notation "'X' x" := (Next x) (at level 65, right associativity) : model_scope.
+Notation "'G' x" := (Globally x) (at level 65, right associativity) : model_scope.
+Notation "'E' x" := (Eventually x) (at level 65, right associativity) : model_scope.
+Notation "x 'U' y" := (Until x y) (at level 60, right associativity) : model_scope.
 
-  Definition matches (s : State) (ss : Seq State) (accs : Seq Action) :=
-    forall (i : nat) (si ssi : State) (ai : Action),
-      nth ss i = Some si ->
-      nth ss (i + 1) = Some ssi ->
-      nth accs i = Some ai ->
-      transition si ai = Some ssi.
+Definition matches (ss : Seq State) (accs : Seq Action) :=
+  forall (i : nat) (si ssi : State) (ai : Action),
+    nth i ss = Some si ->
+    nth (i + 1) ss = Some ssi ->
+    nth i accs = Some ai ->
+    transition si ai = Some ssi.
 
-  Inductive Path := path : forall (s : State) (ss : Seq State) (accs : Seq Action), matches s ss accs -> Path.
+Lemma matches_nth_tl : forall (n : nat) (ss ss_n : Seq State) (accs accs_n : Seq Action), 
+  matches ss accs -> nth_tl n ss = Some ss_n -> nth_tl n accs = Some accs_n -> matches ss_n accs_n.
+Proof.
+  intros.
+  unfold matches.
+  intros.
+  unfold matches in H.
+  specialize (H (n + i) si ssi ai).
+  apply H.
+  - assert (nth ss_n i = nth ss (n + i)). {
+      apply nth_nth_tl.
+      assumption.
+    } 
+    rewrite H5 in H2.
+    assumption.
+  - assert (nth ss_n (i + 1) = nth ss (n + (i + 1))). {
+      apply nth_nth_tl.
+      assumption.
+    }
+    rewrite H5 in H3.
+    assert (n + (i + 1) = n + i + 1) by lia.
+    rewrite H6 in H3.
+    assumption.
+  - assert (nth accs_n i = nth accs (n + i)). {
+      apply nth_nth_tl.
+      assumption.
+    }
+    rewrite H5 in H4.
+    assumption.
+Qed.
 
-  Inductive satisfy : State -> StateFormula -> bool -> Prop :=
-    | satisfyT : forall (s : State), satisfy s true true
-    | satisfyA0 : forall (s : State) (a : atomic),
-        label ts a s = true ->
-        satisfy s (atom a) true
-    | satisfyA1 : forall (s : State) (a : atomic),
-        label ts a s = true ->
-        satisfy s (atom a) true
-    | satisfyNot : forall (s : State) (f : StateFormula), 
-        satisfy s f false -> 
-        satisfy s (not f) true
-    | satisfyAnd : forall (s : State) (f g : StateFormula),
-        satisfy s f true ->
-        satisfy s g true ->
-        satisfy s (conj f g) true
-    | satisfySome : forall (s : State) (p : Path s) (pf : PathFormula),
-        satisfyPath s p pf true ->
-        satisfy s (some pf) true
-    | satisfyEvery : forall (s : State) (pf : PathFormula),
-        (forall (p : Path s), satisfyPath s p pf true) ->
-        satisfy s (every pf) true
-  with satisfyPath : forall s : State, Path s -> PathFormula -> bool -> Prop :=
-    | satisfyNext : forall (s0 s1 : State) (p : Path s1) (a : Action) (f : StateFormula),
-        transition State Action ts s0 a = Some s1 ->
-        satisfy s1 f true ->
-        satisfyPath s0 (pathS s0 s1 p a P) (next f) true
-    | satisfyAlways : forall (s : State) (p : Path s) (f : StateFormula) (i : nat) (si : State),
-      index s p i = Some si -> 
-      satisfy si f true -> 
-      satisfyPath s p (always f) true
-    | satisfyEventually : forall (s : State) (p : Path s) (f : StateFormula),
-      (exists (i : nat) (si : State), index s p i = Some si /\ satisfy si f true) ->
-      satisfyPath s p (eventually f) true
-    | satisfyUntil : forall (s : State) (p : Path s) (f0 f1 : StateFormula), 
-      (exists (j : nat) (sj : State), index s p j = Some sj /\ satisfy sj f1 true /\
-        (forall (k : nat) (sk : State), 
-          k < j ->
-          index s p k = Some sk -> 
-          satisfy sk f0 true)) ->
-      satisfyPath s p (until f0 f1) true.
+Lemma matches_tl : forall (ss ss_tl : Seq State) (accs accs_tl : Seq Action),
+  matches ss accs -> tl ss = Some ss_tl -> tl accs = Some accs_tl -> matches ss_tl accs_tl.
+Proof.
+  intros.
+  apply (matches_nth_tl 1 ss ss_tl accs accs_tl).
+  - assumption.
+  - assert (tl ss = nth_tl ss 1) by apply tl_eq_nth_tl_1.
+    rewrite H2 in H0.
+    assumption.
+  - assert (tl accs = nth_tl accs 1) by apply tl_eq_nth_tl_1.
+    rewrite H2 in H1.
+    assumption.
+Qed.
 
-  Notation "s |= x" := (satisfy s x true) (at level 70, no associativity) : model_scope.
-  Notation "s * p |= x" := (satisfyPath s p x true) (at level 70, no associativity) : model_scope.
+Inductive Path := path : forall (ss : Seq State) (accs : Seq Action), matches ss accs -> Path.
 
-  Lemma infinitely_often : forall (s : State) (f : StateFormula),
-    s |= A F A G f <-> forall p : Path s, exists is : Stream nat, forall (n : nat) (sn : State), index s p (Str_nth n is) = Some sn -> sn |= f.
-  Proof.
-    split.
-    - intros.
-      inversion H.
-      specialize (H2 p).
-      inversion H2.
-      elim H6.
-      intros.
-      elim H7.
-      intros.
-      elim H8.
-      intros.
-      inversion H10.
-  Abort.
+Definition hd_Path (p : Path) :=
+  let (ss, _, _) := p in hd ss.
+
+Definition option_with_eq [A : Type] (x : option A) : option {y : A | x = Some y} := 
+  match x as o return option {y : A | o = Some y} with
+  | Some a => Some (exist (fun y : A => Some a = Some y) a eq_refl)
+  | None => None
+  end.
+
+Definition tl_Path (p : Path) : option Path :=
+  let (ss, accs, P) := p in
+  match option_with_eq (tl ss), option_with_eq (tl accs) with
+  | Some (exist _ ss_tl P_ss_tl), Some (exist _ accs_tl P_accs_tl) =>
+    Some (path ss_tl accs_tl (matches_tl ss ss_tl accs accs_tl P P_ss_tl P_accs_tl))
+  | _, _ => None
+  end.
+
+Definition nth_tl_Path (p : Path) (n : nat) : option Path :=
+  let (ss, accs, P) := p in
+  match option_with_eq (nth_tl ss n), option_with_eq (nth_tl accs n) with
+  | Some (exist _ ss_n P_ss_n), Some (exist _ accs_n P_accs_n) => 
+    Some (path ss_n accs_n (matches_nth_tl n ss ss_n accs accs_n P P_ss_n P_accs_n))
+  | _, _ => None
+  end.
+
+Definition nth_Path (p : Path) (n : nat) :=
+  match nth_tl_Path p n with
+  | Some p' => hd_Path p'
+  | None => None
+  end.
+
+Inductive satisfy : State -> StateFormula -> bool -> Prop :=
+  | satisfyAlways : forall s : State, satisfy s Always true
+  | satisfyAtom : forall (s : State) (a : Atomic), satisfy s (Atom a) (label s a)
+  | satisfyNot : forall (s : State) (f : StateFormula) (b : bool), 
+      satisfy s f b ->
+      satisfy s (Not f) (negb b)
+  | satisfyAnd : forall (s : State) (f0 f1 : StateFormula) (b0 b1 : bool),
+      satisfy s f0 b0 ->
+      satisfy s f1 b1 ->
+      satisfy s (And f0 f1) (b0 && b1)
+  | satisfyExistsTrue : forall (s : State) (pf : PathFormula) (p : Path),
+      hd_Path p = Some s ->
+      satisfyPath p pf true ->
+      satisfy s (Exists pf) true
+  | satisfyExistsFalse : forall (s : State) (pf : PathFormula),
+      (forall (p : Path), hd_Path p = Some s -> satisfyPath p pf false) ->
+      satisfy s (Exists pf) false
+  | satisfyForallTrue : forall (s : State) (pf : PathFormula),
+      (forall (p : Path), hd_Path p = Some s -> satisfyPath p pf true) ->
+      satisfy s (Forall pf) true
+  | satisfyForallFalse : forall (s : State) (pf : PathFormula) (p : Path),
+      hd_Path p = Some s ->
+      satisfyPath p pf false ->
+      satisfy s (Forall pf) false
+with satisfyPath : Path -> PathFormula -> bool -> Prop :=
+  | satisfyNext : forall (p : Path) (f : StateFormula) (sn : State) (b : bool),
+      nth_Path p 1 = Some sn ->
+      satisfy sn f b ->
+      satisfyPath p (Next f) (negb b)
+  | satisfyGloballyTrue : forall (p : Path) (f : StateFormula),
+      (forall (n : nat) (sn : State), nth_Path p n = Some sn -> satisfy sn f true) ->
+      satisfyPath p (Globally f) true
+  | satisfyGloballyFalse : forall (p : Path) (f : StateFormula) (n : nat) (sn : State),
+      nth_Path p n = Some sn -> 
+      satisfy sn f false ->
+      satisfyPath p (Globally f) false
+  | satisfyEventuallyTrue : forall (p : Path) (f : StateFormula) (n : nat) (sn : State),
+      nth_Path p n = Some sn ->
+      satisfy sn f true ->
+      satisfyPath p (Eventually f) true
+  | satisfyEventuallyFalse : forall (p : Path) (f : StateFormula),
+      (forall (n : nat) (sn : State), nth_Path p n = Some sn -> satisfy sn f false) ->
+      satisfyPath p (Eventually f) false
+  | satisfyUntilTrue : forall (p : Path) (f0 f1 : StateFormula) (n : nat) (sn : State),
+      nth_Path p n = Some sn -> 
+      satisfy sn f1 true ->
+      (forall (k : nat) (sk : State), k < n -> nth_Path p k = Some sk -> satisfy sk f0 true) ->
+      satisfyPath p (Until f0 f1) true
+  | satisfyUntilFalse : forall (p : Path) (f0 f1 : StateFormula),
+      (forall (n : nat) (sn : State), nth_Path p n = Some sn -> satisfy sn f1 false \/ (exists (k : nat) (sk : State), k < n -> nth_Path p k = Some sk -> satisfy sk f0 false)) ->
+      satisfyPath p (Until f0 f1) false.
+
+Notation "s |= x" := (satisfy s x true) (at level 70, no associativity) : model_scope.
+Notation "s * p |= x" := (satisfyPath s p x true) (at level 70, no associativity) : model_scope.
+
+Lemma many_often : forall (s : State) (f : StateFormula), s |= Forall E Forall G f <-> 
+  forall p : Path, hd_Path p = Some s -> exists is : Seq nat, forall (n i : nat) (si : State), nth is n = Some i -> nth_Path p i = Some si -> si |= f.
+Proof.
+  intros.
+  split.
+  - intros.
+    inversion H.
+    specialize (H3 p H0).
+    inversion H3.
+    inversion H7.
+    assert (exists pn : Path, nth_tl_Path p n = Some pn). {
+      unfold nth_Path in H5.
+      destruct (nth_tl_Path p n).
+      - exists p1.
+        reflexivity.
+      - discriminate H5.
+    }
+    elim H11.
+    intros.
+    unfold nth_Path in H5.
+    rewrite H12 in H5.
+    specialize (H10 x H5).
+    inversion H10.
+    exists (nats_from n).
+    intros.
+
+Abort.
+
 End Theory.
