Model/Seq.v
@@ -1,4 +1,6 @@
 Set Implicit Arguments.
+Require Import Util.
+Require Import Lia.
 
 Section Seq.
 
@@ -8,32 +10,220 @@ CoInductive Seq :=
   | Nil : Seq
   | Cons : A -> Seq -> Seq.
 
-Definition hd (xs : Seq) :=
-  match xs with
+Definition unfold_seq (s : Seq) := 
+  match s with
+  | Nil => Nil
+  | Cons a tl => Cons a tl
+  end.
+
+Definition hd (s : Seq) :=
+  match s with
   | Nil => None
   | Cons x _ => Some x
   end.
 
-Definition tl (xs : Seq) :=
-  match xs with
+Definition tl (s : Seq) :=
+  match s with
   | Nil => None
   | Cons _ ys => Some ys
   end.
 
-Fixpoint nth_tl (xs : Seq) (n : nat) :=
+Fixpoint nth_tl (n : nat) (s : Seq) :=
   match n with
-  | 0 => Some xs
-  | S m => 
-    match tl xs with
+  | 0 => Some s
+  | S m =>
+    match tl s with
     | None => None
-    | Some ys => nth_tl ys m
+    | Some ys => nth_tl m ys
     end
   end.
 
-Definition nth (xs : Seq) (n : nat) :=
-  match nth_tl xs n with
+Definition nth (n : nat) (s : Seq) :=
+  match nth_tl n s with
   | None => None
   | Some ys => hd ys
   end.
+
+CoFixpoint iterate (f : A -> A) (x : A) := Cons x (iterate f (f x)).
+
+Lemma unfold_seq_eq : forall s, s = unfold_seq s.
+Proof.
+  intros.
+  destruct s.
+  - reflexivity.
+  - reflexivity.
+Qed.
+
+Lemma hd_inv_nil : forall s : Seq, hd s = None -> s = Nil.
+Proof.
+  intros.
+  destruct s.
+  - reflexivity.
+  - discriminate H.
+Qed.
+
+Lemma hd_inv_cons : forall s a, hd s = Some a -> exists s0, s = Cons a s0.
+Proof.
+  intros.
+  destruct s.
+  - discriminate H.
+  - injection H.
+    intros.
+    rewrite H0.
+    exists s.
+    reflexivity.
+Qed.
+
+Lemma tl_inv_nil : forall (s : Seq), tl s = None -> s = Nil.
+Proof.
+  intros.
+  destruct s.
+  - reflexivity.
+  - discriminate H.
+Qed.
+
+Lemma tl_inv_cons : forall (s s0 : Seq), tl s = Some s0 -> exists (a : A), s = Cons a s0.
+Proof.
+  intros.
+  destruct s.
+  - discriminate H.
+  - injection H.
+    intros.
+    rewrite H0.
+    exists a.
+    reflexivity.
+Qed.
+
+Lemma nth_tl_inv_none : forall s n, nth_tl (S n) s = None -> s = Nil \/ exists a s', s = Cons a s' /\ nth_tl n s' = None.
+Proof.
+  intros.
+  destruct s.
+  - left.
+    reflexivity.
+  - right.
+    exists a.
+    exists s.
+    split.
+    * reflexivity.
+    * simpl in H.
+      assumption.
+Qed.
+
+Lemma nth_tl_none_nth_none : forall n s, nth_tl n s = None -> nth n s = None.
+Proof.
+  intros.
+  unfold nth.
+  rewrite H.
+  reflexivity.
+Qed.
+
+Lemma nth_tl_none_plus_m : forall n m s, nth_tl n s = None -> nth_tl (m + n) s = None.
+Proof.
+  intros n m.
+  destruct m.
+  - intros.
+    simpl.
+    assumption.
+  - induction n.
+    * intros.
+      discriminate H.
+    * intros.
+      pose proof (nth_tl_inv_none s n H).
+      elim H0.
+      + intros.
+        rewrite H1.
+        reflexivity.
+      + intros.
+        elim H1.
+        intros.
+        elim H2.
+        intros.
+        elim H3.
+        intros.
+        rewrite H4.
+        simpl.
+        assert (m + S n = S m + n) by lia.
+        rewrite H6.
+        apply IHn.
+        assumption.
+Qed.
+
+Lemma tl_nth_tl : forall (n : nat) (s : Seq), x <- nth_tl n s ;; tl x = x <- tl s ;; nth_tl n x.
+Proof.
+  intro n.
+  induction n.
+  - intros.
+    destruct s.
+    * reflexivity.
+    * reflexivity.
+  - intros.
+    destruct s.
+    * reflexivity.
+    * simpl.
+      specialize (IHn s).
+      destruct (tl s).
+      + simpl in IHn.
+        assumption.
+      + simpl in IHn.
+        assumption.
+Qed.
+
+Lemma nth_nth_tl : forall (n m : nat) (s : Seq), x <- nth_tl n s ;; nth m x = nth (m + n) s.
+Proof.
+  intros.
+  apply bind_eq.
+  - intros.
+    apply nth_tl_none_nth_none.
+    apply nth_tl_none_plus_m.
+    assumption.
+  - intro a.
+    generalize s.
+    induction n.
+    * intros.
+      injection H.
+      intros.
+      rewrite H0.
+      assert (m + 0 = m) by lia.
+      rewrite H1.
+      reflexivity.
+    * intros.
+      destruct s0.
+      + discriminate H.
+      + simpl in H.
+        pose proof (IHn s0 H).
+        assert (m + S n = S (m + n)) by lia.
+        rewrite H1.
+        unfold nth.
+        simpl.
+        unfold nth in H0.
+        assumption.
+Qed.
+
+Fixpoint n_compose (n : nat) (f : A -> A) : A -> A :=
+  match n with
+  | 0 => id
+  | S m => fun x => f (n_compose m f x)
+  end.
+
+Lemma iterate_nth : forall n x f, nth n (iterate f x) = Some (n_compose n f x).
+Proof.
+  intro n.
+  induction n.
+  - intros.
+    pattern (iterate f x).
+    rewrite unfold_seq_eq.
+    simpl. 
+    unfold nth.
+    unfold id.
+    reflexivity.
+  - intros.
+    pattern (iterate f x).
+    rewrite unfold_seq_eq.
+    simpl.
+    unfold nth.
+    simpl.
+    pose proof (IHn (f x) f).
+    unfold nth in H.
+Qed.
 
 End Seq.
