Model/Util.v
@@ -1,0 +1,29 @@
+Set Implicit Arguments.
+Declare Scope util_scope.
+Open Scope util_scope.
+
+Definition bind [A B : Type] (x : option A) (f : A -> option B) : option B :=
+  match x with
+  | None => None
+  | Some a => f a
+  end.
+
+Notation "x >>= f" := (bind x f) (at level 58, left associativity) : util_scope.
+Notation "x >> y" := (bind x (fun _ => y)) (at level 58, left associativity) : util_scope.
+Notation "x <- y ;; z" := (y >>= (fun x => z)) (at level 61, y at next level, right associativity) : util_scope.
+Notation "x ;; z" := (x >> z) (at level 61, right associativity) : util_scope.
+
+Lemma bind_eq : forall [A B : Type] (x : option A) (f : A -> option B) (y : option B), 
+  (x = None -> y = None) ->
+  (forall a : A, Some a = x -> f a = y) ->
+  x >>= f = y.
+Proof.
+  intros.
+  unfold bind.
+  destruct x.
+  - apply H0.
+    reflexivity.
+  - symmetry.
+    apply H.
+    reflexivity.
+Qed.
